going locally nameless, with quite a lot of bureaucracy

examples/dsls/stlc/STLC.fst
@@ -8,19 +8,74 @@ type stlc_ty =
   | TArrow : stlc_ty -> stlc_ty -> stlc_ty
 
 let var = nat
+let index = nat
 
-let tun = R.(pack_ln Tv_Unknown)
+assume
+val close (t:R.term) : R.term
+
+let tun = R.pack_ln R.Tv_Unknown
 
 noeq
 type stlc_exp (t:Type) =
   | EUnit : stlc_exp t
+  | EBVar : index -> stlc_exp t
   | EVar  : var -> stlc_exp t
   | ELam  : t -> stlc_exp t -> stlc_exp t
   | EApp  : stlc_exp t -> stlc_exp t -> stlc_exp t
 
-let s_exp = stlc_exp stlc_ty
-let stlc_env = list stlc_ty
+let rec size (e:stlc_exp 'a) 
+  : nat
+  = match e with
+    | EUnit
+    | EBVar _ 
+    | EVar _ -> 1
+    | ELam _ e -> 1 + size e
+    | EApp e1 e2 -> 1 + size e1 + size e2
+    
+let rec open_exp' (e:stlc_exp 'a) (v:var) (n:index)
+  : e':stlc_exp 'a { size e == size e'}
+  = match e with
+    | EUnit -> EUnit
+    | EVar m -> EVar m
+    | EBVar m -> if m = n then EVar v else EBVar m
+    | ELam t e -> ELam t (open_exp' e v (n + 1))
+    | EApp e1 e2 -> EApp (open_exp' e1 v n) (open_exp' e2 v n)
 
+let rec close_exp' (e:stlc_exp 'a) (v:var) (n:nat)
+  : e':stlc_exp 'a { size e == size e'}
+  = match e with
+    | EUnit -> EUnit
+    | EVar m -> if m = v then EBVar n else EVar m
+    | EBVar m -> EBVar m
+    | ELam t e -> ELam t (close_exp' e v (n + 1))
+    | EApp e1 e2 -> EApp (close_exp' e1 v n) (close_exp' e2 v n)
+
+let open_exp e v = open_exp' e v 0
+let close_exp e v = close_exp' e v 0
+
+let open_close (e:stlc_exp 'a) (x:var)
+  : Lemma (open_exp (close_exp e x) x == e)
+          [SMTPat (open_exp (close_exp e x) x)]
+  = admit()
+  
+let s_exp = stlc_exp stlc_ty
+
+let stlc_env = list (var & stlc_ty)
+
+let lookup (e:list (var & 'a)) (x:var)
+  : option 'a
+  = L.assoc x e
+
+let max (n1 n2:nat) = if n1 < n2 then n2 else n1
+
+let fresh (e:list (var & 'a))
+  : var
+  = L.fold_right (fun (n, _) v -> max v n) e 0 + 1
+
+let fresh_is_fresh (e:list (var & 'a))
+  : Lemma (None? (lookup e (fresh e)))
+  = admit()
+  
 [@@erasable]
 noeq
 type stlc_typing : stlc_env -> s_exp -> stlc_ty -> Type =
@@ -30,15 +85,16 @@ type stlc_typing : stlc_env -> s_exp -> stlc_ty -> Type =
   
   | T_Var  :
       g:stlc_env ->
-      x:var { Some? (L.nth g x) } ->
-      stlc_typing g (EVar x) (Some?.v (L.nth g x))
+      x:var { Some? (lookup g x) } ->
+      stlc_typing g (EVar x) (Some?.v (lookup g x))
 
   | T_Lam  :
       g:stlc_env ->
       t:stlc_ty ->
       e:s_exp ->
       t':stlc_ty ->
-      stlc_typing (t::g) e t' ->
+      x:var { x == fresh g } ->
+      stlc_typing ((x,t)::g) (open_exp e x) t' ->
       stlc_typing g (ELam t e) (TArrow t t')
 
   | T_App  :
@@ -63,62 +119,73 @@ let rec elab_ty (t:stlc_ty)
     | TArrow t1 t2 ->
       let t1 = elab_ty t1 in
       let t2 = elab_ty t2 in
-//      let bv = R.pack_bv ({ bv_ppname = ""; bv_index = 0; bv_sort = t1 }) in
+
       R.pack_ln 
         (R.Tv_Arrow 
           (RT.as_binder 0 t1)
-//          (R.pack_binder bv R.Q_Explicit [])
           (R.pack_comp (C_Total t2 [])))
 
 let make_bv (n:nat) (t:R.term) = R.({ bv_ppname = ""; bv_index = n; bv_sort = t})
 let bv_as_binder bv = R.pack_binder bv R.Q_Explicit []
-
-let rec elab_exp (e:s_exp)
-  : R.term
+let bv_index_of_make_nv (n:nat) (t:R.term)
+  : Lemma (ensures RT.bv_index (R.pack_bv (make_bv n t)) == n)
+          [SMTPat (RT.bv_index (R.pack_bv (make_bv n t)))]
+  = admit()
+  
+let rec elab_exp (g:stlc_env) (e:s_exp)
+  : Tot R.term (decreases (size e))
   = let open R in
     match e with
     | EUnit -> 
       pack_ln (Tv_Const C_Unit)
 
+    | EBVar n -> 
+      let bv = R.pack_bv (make_bv n tun) in
+      R.pack_ln (Tv_BVar bv)
+      
     | EVar n ->
       // tun because type does not matter at a use site
       let bv = R.pack_bv (make_bv n tun) in
-      R.pack_ln (Tv_BVar bv)
+      R.pack_ln (Tv_Var bv)
 
     | ELam t e ->
+      let x = fresh g in 
+      let g' = (x, t) :: g in
       let t = elab_ty t in
-      let e = elab_exp e in
-      R.pack_ln (Tv_Abs (RT.as_binder 0 t) e)
+      let e = elab_exp g' (open_exp e x) in
+      R.pack_ln (Tv_Abs (RT.as_binder 0 t) (RT.close_term e x))
              
     | EApp e1 e2 ->
-      let e1 = elab_exp e1 in
-      let e2 = elab_exp e2 in
+      let e1 = elab_exp g e1 in
+      let e2 = elab_exp g e2 in
       R.pack_ln (Tv_App e1 (e2, Q_Explicit))
-
-
 
 let new_hole (g:R.env)
   : T.Tac R.term
   = T.uvar_env g (Some (`stlc_ty))
     
 let rec infer (g:R.env)
-              (sg:list R.term)
+              (sg:list (var & R.term))
               (e:stlc_exp unit)
   : T.Tac (stlc_exp R.term & R.term)
   = match e with
     | EUnit ->
       EUnit, `TUnit
+
+    | EBVar _ -> 
+      T.fail "Locally nameless"
       
     | EVar x ->
       begin
-      match L.nth sg x with
+      match lookup sg x with
       | None -> T.fail "Unbound variable"
       | Some ht -> EVar x, ht
       end
 
     | ELam _ e ->
       let t0 = new_hole g in
-      let e, t = infer g (t0 :: sg) e in
+      let x = fresh sg in
+      let e, t = infer g ((x, t0) :: sg) (open_exp e x) in
       ELam t e, `(TArrow (`#(t0)) (`#(t)))
 
     | EApp e1 e2 ->
@@ -170,7 +237,7 @@ let rec read_back (g:R.env) (t:R.term)
       T.fail "Unexpected constructor of stlc_ty"
   
 let rec check (g:R.env)
-              (sg:list stlc_ty)
+              (sg:list (var & stlc_ty))
               (e:stlc_exp R.term)
   : T.Tac (e':s_exp &
            t':stlc_ty &
@@ -179,10 +246,13 @@ let rec check (g:R.env)
     | EUnit ->
       let d = T_Unit sg in
       (| EUnit, TUnit, d |)
+      
+    | EBVar _ -> 
+      T.fail "Locally nameless"
 
     | EVar n ->
       begin
-      match L.nth sg n with
+      match lookup sg n with
       | None -> T.fail "Ill-typed"
       | Some t ->
         let d = T_Var sg n in
@@ -190,11 +260,13 @@ let rec check (g:R.env)
       end
 
     | ELam rt e ->
+      let x = fresh sg in
+      fresh_is_fresh sg;
       let t = read_back g rt in
-      let (| e, tbody, dbody |) = check g (t::sg) e in
-      (| ELam t e, 
+      let (| e, tbody, dbody |) = check g ((x,t)::sg) (open_exp e x) in
+      (| ELam t (close_exp e x), 
          TArrow t tbody, 
-         T_Lam sg t e tbody dbody |)
+         T_Lam sg t (close_exp e x) tbody x dbody |)
            
     | EApp e1 e2 ->
       let (| e1, t1, d1 |) = check g sg e1  in
@@ -217,7 +289,17 @@ let infer_and_check (g:R.env)
     (| e'', t' |)
 
 let extend_env_l (g:R.env) (sg:stlc_env) = 
-  L.fold_left (fun g t -> RT.extend_env g 0 (elab_ty t)) g sg
+  L.fold_left (fun g (x, t) -> RT.extend_env g x (elab_ty t)) g sg
+
+let extend_env_l_lookup_bvar (g:R.env) (sg:stlc_env) (x:var)
+  : Lemma 
+    (requires (forall x. RT.lookup_bvar g x == None))
+    (ensures (
+      match lookup sg x with
+      | Some t -> RT.lookup_bvar (extend_env_l g sg) x == Some (elab_ty t)
+      | None -> RT.lookup_bvar (extend_env_l g sg) x == None))
+    [SMTPat (RT.lookup_bvar (extend_env_l g sg) x)]
+  = admit()
 
 let binder_sort_lemma (x:R.var) (ty:R.term)
   : Lemma (RT.binder_sort (RT.as_binder x ty) == ty)
@@ -234,35 +316,70 @@ let rec soundness (#sg:stlc_env)
                   (#se:s_exp)
                   (#st:stlc_ty)
                   (dd:stlc_typing sg se st)
-                  (g:R.env)
+                  (g:R.env { forall x. None? (RT.lookup_bvar g x) } )
   : GTot (RT.typing (extend_env_l g sg)
-                    (elab_exp se)
+                    (elab_exp sg se)
                     (elab_ty st))
+         (decreases dd)
   = match dd with
     | T_Unit _ ->
       RT.T_Const _
 
-    | T_Var _ x -> admit()
+    | T_Var _ x ->
+      RT.T_Var _ (R.pack_bv (make_bv x tun))
 
-    | T_Lam _ t e t' de -> admit()
+    | T_Lam _ t e t' x de ->
+      let de : RT.typing (extend_env_l g ((x,t)::sg))
+                         (elab_exp ((x,t)::sg) (open_exp e x))
+                         (elab_ty t')
+            = soundness de g 
+      in    
+      assume ((extend_env_l g ((x,t)::sg)) == RT.extend_env (extend_env_l g sg) x (elab_ty t)); //easy
+      assume (RT.close_term (elab_ty t') x == elab_ty t'); //A property of STLC type elaborations 
+      //opening and then elaborating, elaborating and then opening
+      assume ((elab_exp ((x,t)::sg) (open_exp e x)) == RT.open_term (elab_exp ((x,t)::sg) e) x);
+      let de : RT.typing (RT.extend_env (extend_env_l g sg) x (elab_ty t))
+                         (elab_exp ((x,t)::sg) (open_exp e x))
+                         (elab_ty t')
+             = de
+      in
+      fresh_is_fresh sg;
+      let dd
+        : RT.typing (extend_env_l g sg)
+                    (R.pack_ln (R.Tv_Abs (RT.as_binder 0 (elab_ty t)) (elab_exp ((x,t)::sg) e)))
+                    (elab_ty (TArrow t t'))
+        = RT.T_Abs (extend_env_l g sg)
+                   x
+                   (elab_ty t) (elab_exp ((x,t)::sg) e) (elab_ty t') de
+      in
+      calc (==) {
+       elab_exp sg (ELam t e);
+      == {}
+       R.pack_ln (R.Tv_Abs (RT.as_binder 0 (elab_ty t)) (RT.close_term (elab_exp ((x, t)::sg) (open_exp e x)) x)); 
+      == { //opening, elaborating, closing ... open/close cancel across the elab 
+           assume ((RT.close_term (elab_exp ((x, t)::sg) (open_exp e x)) x) == (elab_exp ((x,t)::sg) e))
+         }
+       R.pack_ln (R.Tv_Abs (RT.as_binder 0 (elab_ty t)) (elab_exp ((x, t)::sg) e));
+      };
+      dd
     
     | T_App _ e1 e2 t t' d1 d2 ->
       let dt1 
         : RT.typing (extend_env_l g sg)
-                    (elab_exp e1)
+                    (elab_exp sg e1)
                     (elab_ty (TArrow t t'))
         = soundness d1 g
       in
       let dt2
         : RT.typing (extend_env_l g sg)
-                    (elab_exp e2)
+                    (elab_exp sg e2)
                     (elab_ty t)
         = soundness d2 g
       in
       let dt :
         RT.typing (extend_env_l g sg)
-                  (elab_exp (EApp e1 e2))
-                  (RT.open_with (elab_ty t') (elab_exp e2))
+                  (elab_exp sg (EApp e1 e2))
+                  (RT.open_with (elab_ty t') (elab_exp sg e2))
         = RT.T_App _ _ _ _ _ dt1 dt2
       in
       dt
@@ -270,21 +387,20 @@ let rec soundness (#sg:stlc_env)
 let soundness_lemma (sg:stlc_env) 
                     (se:s_exp)
                     (st:stlc_ty)
-                    (g:R.env)  
-                  
-  
+                    (g:R.env { forall x. None? (RT.lookup_bvar g x ) })                   
   : Lemma
     (requires stlc_typing sg se st)
     (ensures  RT.typing (extend_env_l g sg)
-                        (elab_exp se)
+                        (elab_exp sg se)
                         (elab_ty st))
   = FStar.Squash.bind_squash 
       #(stlc_typing sg se st)
       ()
       (fun dd -> FStar.Squash.return_squash (soundness dd g))
 
-let main (g:R.env) (src:stlc_exp unit)
+let main (g:R.env { forall x. None? (RT.lookup_bvar g x ) })
+         (src:stlc_exp unit)
   : T.Tac (e:R.term & t:R.term { RT.typing g e t })
   = let (| src', src_ty |) = infer_and_check g src in
     soundness_lemma [] src' src_ty g;
-    (| elab_exp src', elab_ty src_ty |)
+    (| elab_exp [] src', elab_ty src_ty |)
