examples/dsls/stlc/Refl.Typing.fsti
@@ -1,0 +1,62 @@
+module Refl.Typing
+open FStar.Reflection
+
+val lookup_bvar (e:env) (x:int) : option term
+
+val lookup_fvar (e:env) (x:fv) : option term
+
+val extend_env (e:env) (x:var) (ty:term) : env
+
+//replace BV 0 in t with v
+val open_with (t:term) (v:term) : term
+val open_term (t:term) (v:var) : term
+val close_term (t:term) (v:var) : term
+let as_binder (x:var) (ty:term)
+  : binder 
+  = pack_binder
+      (pack_bv ({bv_ppname="";
+                 bv_index=x;
+                 bv_sort=ty}))
+      Q_Explicit
+      []
+
+let bv_index (x:bv) : int = (inspect_bv x).bv_index
+  
+let unit_exp = pack_ln (Tv_Const C_Unit)
+let unit_ty = pack_ln (Tv_FVar (pack_fv unit_lid))
+let binder_sort (b:binder) =
+  let bv, _ = inspect_binder b in 
+  (inspect_bv bv).bv_sort
+    
+noeq
+type typing : env -> term -> term -> Type0 =
+  | T_Var : 
+     g:env ->
+     x:bv { Some? (lookup_bvar g (bv_index x)) } ->
+     typing g (pack_ln (Tv_Var x)) (Some?.v (lookup_bvar g (bv_index x)))
+
+  | T_Const:
+     g:env ->
+     typing g unit_exp unit_ty
+
+  | T_Abs :
+     g:env ->
+     x:var { None? (lookup_bvar g x) } ->
+     ty:term ->
+     body:term ->
+     body_ty:term ->
+     typing (extend_env g x ty) (open_term body x) body_ty ->
+     typing g (pack_ln (Tv_Abs (as_binder 0 ty) body))
+              (pack_ln (Tv_Arrow (as_binder 0 ty) 
+                                 (pack_comp (C_Total (close_term body_ty x) []))))
+
+  | T_App :
+     g:env ->
+     e1:term ->
+     e2:term ->
+     x:binder ->
+     t:term ->
+     typing g e1 (pack_ln (Tv_Arrow x (pack_comp (C_Total t [])))) ->
+     typing g e2 (binder_sort x) ->
+     typing g (pack_ln (Tv_App e1 (e2, Q_Explicit)))
+              (open_with t e2)
